Add std_queue.

theories/std/queue.v
@@ -1,9 +1,12 @@
 From caml5 Require Import
   prelude.
 From caml5.lang Require Import
-  notations.
+  notations
+  proofmode.
 From caml5.std Require Export
   base.
+From caml5.std Require Import
+  chain.
 
 Record queue `{!heapGS Σ} := {
   queue_make : val ;
@@ -43,3 +46,150 @@ Record queue `{!heapGS Σ} := {
 #[global] Arguments queue _ {_} : assert.
 #[global] Arguments Build_queue {_ _ _ _ _ _ _ _} _ _ _ _ : assert.
 #[global] Existing Instance queue_model_timeless.
+
+Section std_queue.
+  Context `{!heapGS Σ}.
+  Implicit Types l : loc.
+  Implicit Types t v hd tl : val.
+
+  Notation queue_offset_head := 0%Z.
+  Notation queue_offset_tail := 1%Z.
+
+  Notation "t '.(head)'" := (t +ₗ queue_offset_head)%stdpp
+  ( at level 5
+  ) : stdpp_scope.
+  Notation "t '.(tail)'" := (t +ₗ queue_offset_tail)%stdpp
+  ( at level 5
+  ) : stdpp_scope.
+  Notation "t '.(head)'" := (t +ₗ #queue_offset_head)%E
+  ( at level 5
+  ) : expr_scope.
+  Notation "t '.(tail)'" := (t +ₗ #queue_offset_tail)%E
+  ( at level 5
+  ) : expr_scope.
+
+  Definition std_queue_make : val :=
+    λ: <>,
+      let: "tl" := chain_cons #() #() in
+      AllocN #2 "tl".
+
+  Definition std_queue_is_empty : val :=
+    λ: "t",
+      !"t".(head) = !"t".(tail).
+
+  Definition std_queue_push : val :=
+    λ: "t" "v",
+      let: "tl" := chain_cons #() #() in
+      chain_set_head !"t".(tail) "v" ;;
+      chain_set_tail !"t".(tail) "tl" ;;
+      "t".(tail) <- "tl".
+
+  Definition std_queue_pop : val :=
+    λ: "t",
+      if: std_queue_is_empty "t" then (
+        NONE
+      ) else (
+        let: "v" := chain_head !"t".(head) in
+        "t".(head) <- chain_tail !"t".(head) ;;
+        SOME "v"
+      ).
+
+  Definition std_queue_model t vs : iProp Σ :=
+    ∃ l hd tl,
+    ⌜t = #l⌝ ∗
+    l.(head) ↦ hd ∗ l.(tail) ↦ tl ∗
+    chain_model hd (DfracOwn 1) (reverse vs) tl ∗ chain_model tl (DfracOwn 1) [ #()] #().
+
+  #[global] Instance std_queue_model_timeless t vs :
+    Timeless (std_queue_model t vs).
+  Proof.
+    apply _.
+  Qed.
+
+  Lemma std_queue_make_spec :
+    {{{ True }}}
+      std_queue_make #()
+    {{{ t, RET t; std_queue_model t [] }}}.
+  Proof.
+    iIntros "%Φ _ HΦ".
+    wp_rec.
+    wp_apply (chain_cons_spec _ (DfracOwn 1)); [done | by iApply chain_model_nil |]. iIntros "%tl Htl_model".
+    wp_pures. wp_alloc l as "Hl"; first done.
+    iDestruct (array_cons with "Hl") as "(Hhd & Htl)".
+    iEval (setoid_rewrite <- loc_add_0) in "Hhd".
+    iDestruct (array_singleton with "Htl") as "Htl".
+    iModIntro. iApply "HΦ". iExists l, tl, tl. iFrame. iSplit; [done | by iApply chain_model_nil].
+  Qed.
+
+  Lemma std_queue_is_empty_spec t vs :
+    {{{ std_queue_model t vs }}}
+      std_queue_is_empty t
+    {{{ RET #(bool_decide (vs = [])); std_queue_model t vs }}}.
+  Proof.
+    iIntros "%Φ (%l & %hd & %tl & -> & Hhd & Htl & Hhd_model & Htl_model) HΦ".
+    wp_rec. wp_pures. wp_load. wp_pures. wp_load.
+    destruct vs as [| v vs].
+    - iDestruct (chain_model_nil with "Hhd_model") as %->.
+      iDestruct (chain_model_unboxed with "Htl_model") as %?.
+      wp_pures.
+      iEval (rewrite bool_decide_eq_true_2). iApply "HΦ". iExists l, tl, tl. auto with iFrame.
+    - iDestruct (chain_model_unboxed with "Htl_model") as %?.
+      wp_pures.
+      iDestruct (chain_model_ne with "Htl_model Hhd_model") as %?; first (rewrite reverse_length /=; lia).
+      rewrite (bool_decide_eq_false_2 (hd = tl)); last done.
+      iApply "HΦ". iExists l, hd, tl. auto with iFrame.
+  Qed.
+
+  Lemma std_queue_push_spec t vs v :
+    {{{ std_queue_model t vs }}}
+      std_queue_push t v
+    {{{ RET #(); std_queue_model t (v :: vs) }}}.
+  Proof.
+    iIntros "%Φ (%l & %hd & %tl & -> & Hhd & Htl & Hhd_model & Htl_model) HΦ".
+    wp_rec. wp_pures.
+    wp_apply (chain_cons_spec _ (DfracOwn 1)); [done | by iApply chain_model_nil |]. iIntros "%tl' Htl'_model".
+    wp_pures. wp_load.
+    wp_apply (chain_set_head_spec with "Htl_model"). iIntros "Htl_model".
+    wp_pures. wp_load.
+    wp_apply (chain_set_tail_spec with "Htl_model"). iIntros "%_ (Htl_model & _)".
+    iDestruct (chain_model_app_1 with "Hhd_model Htl_model") as "Hhd_model".
+    rewrite -reverse_cons.
+    wp_pures. wp_store.
+    iModIntro. iApply "HΦ". iExists l, hd, tl'. auto with iFrame.
+  Qed.
+
+  Lemma std_queue_pop_spec t vs :
+    {{{ std_queue_model t vs }}}
+      std_queue_pop t
+    {{{ w,
+      RET w;
+      (⌜vs = [] ∧ w = NONEV⌝ ∗ std_queue_model t []) ∨
+      (∃ vs' v, ⌜vs = vs' ++ [v] ∧ w = SOMEV v⌝ ∗ std_queue_model t vs')
+    }}}.
+  Proof.
+    iIntros "%Φ Hmodel HΦ".
+    wp_rec.
+    wp_apply (std_queue_is_empty_spec with "Hmodel"). iIntros "(%l & %hd & %tl & -> & Hhd & Htl & Hhd_model & Htl_model)".
+    destruct (reverse vs) as [| v rev_vs] eqn:Heq;
+      apply (f_equal reverse) in Heq; rewrite reverse_involutive in Heq; subst;
+      wp_pures.
+    { iModIntro. iApply "HΦ". iLeft. iSplit; first done. iExists l, hd, tl. auto with iFrame. }
+    rewrite reverse_cons bool_decide_eq_false_2; last eauto using app_cons_not_nil.
+    wp_pures. wp_load.
+    wp_apply (chain_head_spec with "Hhd_model"). iIntros "Hhd_model".
+    wp_pures. wp_load.
+    wp_apply (chain_tail_spec with "Hhd_model"). iIntros "%hd' (Hhd_model & Hhd'_model)".
+    wp_store. wp_pures.
+    iModIntro. iApply "HΦ". iRight. iExists (reverse rev_vs), v. iSplit; first done.
+    iExists l, hd', tl. rewrite reverse_involutive. auto with iFrame.
+  Qed.
+
+  Definition std_queue : queue Σ :=
+    Build_queue
+      std_queue_make_spec
+      std_queue_is_empty_spec
+      std_queue_push_spec
+      std_queue_pop_spec.
+End std_queue.
+
+#[global] Typeclasses Opaque std_queue_model.
